src/program_proof/simplepb/pb_becomeprimary_proof.v
@@ -1,0 +1,302 @@
+From Perennial.program_proof Require Import grove_prelude.
+From Goose.github_com.mit_pdos.gokv.simplepb Require Export pb.
+From Perennial.program_proof.grove_shared Require Import urpc_proof urpc_spec.
+From Perennial.program_proof.simplepb Require Export pb_ghost.
+From Perennial.program_proof.simplepb Require Import pb_marshal_proof.
+From Perennial.program_proof Require Import marshal_stateless_proof.
+From Perennial.program_proof.simplepb Require Import pb_definitions pb_makeclerk_proof.
+
+(* FIXME: for `list_copy_one_more_element` *)
+From Perennial.program_proof.simplepb Require Import config_marshal_proof.
+
+Section pb_becomeprimary_proof.
+Context `{!heapGS Σ, !stagedG Σ}.
+Context {pb_record:PBRecord}.
+
+Notation OpType := (pb_OpType pb_record).
+Notation has_op_encoding := (pb_has_op_encoding pb_record).
+Notation has_snap_encoding := (pb_has_snap_encoding pb_record).
+Notation has_op_encoding_injective := (pb_has_op_encoding_injective pb_record).
+Notation compute_reply := (pb_compute_reply pb_record).
+Notation pbG := (pbG (pb_record:=pb_record)).
+
+Context `{!waitgroupG Σ}.
+Context `{!pbG Σ}.
+
+Lemma wp_Clerk__BecomePrimary γ γsrv ck args_ptr args σ backupγ:
+  {{{
+        "#Hck" ∷ is_Clerk ck γ γsrv ∗
+        "#Hconf" ∷ is_epoch_config γ args.(BecomePrimaryArgs.epoch) ([γsrv] ++ backupγ) ∗
+        (* FIXME: want this to be "is_pb_host", but that will require recursion *)
+        "#Hhosts" ∷ ([∗ list] host ; γsrv' ∈ args.(BecomePrimaryArgs.replicas) ; [γsrv] ++ backupγ, True) ∗
+        "#Hprop_lb" ∷ is_proposal_lb γ args.(BecomePrimaryArgs.epoch) σ ∗
+        "#Hprop_facts" ∷ is_proposal_facts γ args.(BecomePrimaryArgs.epoch) σ ∗
+        "#Hprim_escrow" ∷ become_primary_escrow γ γsrv args.(BecomePrimaryArgs.epoch) σ ∗
+        "Hargs" ∷ BecomePrimaryArgs.own args_ptr args
+  }}}
+    Clerk__BecomePrimary #ck #args_ptr
+  {{{
+        (err:u64), RET #err; True
+  }}}.
+Proof.
+  iIntros (Φ) "Hpre HΦ".
+  iNamed "Hpre".
+  wp_call.
+  wp_apply (wp_ref_of_zero).
+  { done. }
+  iIntros (rep) "Hrep".
+  wp_pures.
+  iNamed "Hck".
+  wp_apply (BecomePrimaryArgs.wp_Encode with "[$Hargs]").
+  iIntros (enc_args enc_args_sl) "(%Henc_args & Henc_args_sl & Hargs)".
+  wp_loadField.
+  iDestruct (is_slice_to_small with "Henc_args_sl") as "Henc_args_sl".
+  wp_apply (wp_frame_wand with "HΦ").
+  wp_apply (wp_Client__Call2 with "Hcl_rpc [] Henc_args_sl Hrep").
+  {
+    iDestruct "Hsrv" as "[_ [_ [_ [$ _]]]]".
+  }
+  { (* Successful RPC *)
+    iModIntro.
+    iNext.
+    unfold BecomePrimary_spec.
+    iExists _, _, _.
+    iSplitR; first done.
+    iSplitR; first done.
+    simpl.
+    iFrame "Hhosts".
+    iFrame "Hprop_lb Hprop_facts Hprim_escrow".
+    (* BecomePrimary was rejected by the server (e.g. stale epoch number) *)
+    iIntros (err) "%Herr_nz".
+    iIntros.
+    wp_pures.
+    wp_load.
+    wp_call.
+    rewrite H.
+    wp_apply (wp_ReadInt with "[$]").
+    iIntros.
+    wp_pures.
+    iModIntro.
+    iIntros "HΦ".
+    iApply "HΦ".
+    done.
+  }
+  { (* RPC error *)
+    iIntros.
+    wp_pures.
+    wp_if_destruct.
+    {
+      iModIntro.
+      iIntros "HΦ".
+      iApply "HΦ".
+      done.
+    }
+    { exfalso. done. }
+  }
+Qed.
+
+Lemma wp_Server__BecomePrimary γ γsrv s args_ptr args σ backupγ Φ :
+  is_Server s γ γsrv -∗
+  BecomePrimaryArgs.own args_ptr args -∗
+  BecomePrimary_core_spec γ γsrv args σ backupγ (λ err, Φ #err) -∗
+  WP pb.Server__BecomePrimary #s #args_ptr {{ Φ }}
+  .
+Proof.
+  iIntros "#His_srv Hargs HΦ".
+  iNamed "His_srv".
+  wp_call.
+  wp_loadField.
+  wp_apply (acquire_spec with "[$HmuInv]").
+  iIntros "[Hlocked Hown]".
+  wp_pures.
+  iNamed "Hown".
+  iNamed "Hargs".
+  wp_loadField.
+
+  iDestruct "HΦ" as "(#Hconf & #Hhosts & #Hprimary_escrow & Hprimary_facts & Hprimary_lb & HΦ)".
+
+  wp_call.
+  wp_loadField.
+  wp_if_destruct.
+  { (* stale epoch *)
+    wp_loadField.
+    unfold BecomePrimary_core_spec.
+    wp_apply (release_spec with "[-HΦ]").
+    {
+      iFrame "HmuInv Hlocked".
+      iNext.
+      iExists _, _, _, _, _, _, _.
+      iFrame "∗#%".
+    }
+    wp_pures.
+    iApply "HΦ".
+  }
+  { (* successfully become primary *)
+    wp_storeField.
+    wp_loadField.
+    wp_apply (wp_slice_len).
+    wp_apply (wp_NewSlice).
+    iIntros (new_clerks_sl) "Hnew_clerks_sl".
+    iDestruct (is_slice_to_small with "Hnew_clerks_sl") as "Hnew_clerks_sl".
+    wp_storeField.
+    wp_apply (wp_ref_to).
+    { eauto. }
+    iIntros (i_ptr) "Hi".
+    wp_pures.
+
+    iDestruct (is_slice_small_sz with "Hargs_replicas_sl") as %Hreplicas_sz.
+    iDestruct (big_sepL2_length with "Hhosts") as %Hreplicas_backup_len.
+
+    iAssert (
+          ∃ (i:u64) clerksComplete clerksLeft,
+            "Hi" ∷ i_ptr ↦[uint64T] #i ∗
+            "%HcompleteLen" ∷ ⌜length clerksComplete = int.nat i⌝ ∗
+            "%Hlen" ∷ ⌜length (clerksComplete ++ clerksLeft) = length backupγ⌝ ∗
+            "Hclerks_sl" ∷ is_slice_small new_clerks_sl ptrT 1 (clerksComplete ++ clerksLeft) ∗
+            "Hreplicas_sl" ∷ is_slice_small replicas_sl uint64T 1 args.(BecomePrimaryArgs.replicas) ∗
+            "#Hclerks_is" ∷ ([∗ list] ck ; γsrv ∈ clerksComplete ; (take (length clerksComplete) backupγ),
+                                pb_definitions.is_Clerk ck γ γsrv
+                                )
+            )%I with "[Hnew_clerks_sl Hargs_replicas_sl Hi]" as "HH".
+    {
+      iExists _, [], _.
+      simpl.
+      iFrame "∗#".
+      iPureIntro.
+      split; first word.
+      rewrite replicate_length.
+      rewrite app_length /= in Hreplicas_backup_len.
+      word.
+    }
+
+    wp_forBreak_cond.
+    iNamed "HH".
+
+    wp_pures.
+    wp_load.
+    wp_loadField.
+    wp_apply (wp_slice_len).
+    wp_if_destruct.
+    { (* continue with loop *)
+      assert (int.nat i < length backupγ) as Hi.
+      {
+        rewrite app_length /= Hreplicas_sz in Hreplicas_backup_len.
+        admit. (* TODO: word *)
+      }
+      pose proof Hi as Hlookup.
+      apply list_lookup_lt in Hlookup as [γsrv' Hlookup].
+      assert (([γsrv] ++ backupγ) !! (int.nat i + 1) = Some γsrv').
+      {
+        rewrite lookup_app_r.
+        {
+          simpl. rewrite -Hlookup.
+          f_equal. word.
+        }
+        {
+          simpl. word.
+        }
+      }
+      iDestruct (big_sepL2_lookup_2_some with "Hhosts") as "%Hlookup_replicas".
+      {
+        done.
+      }
+      destruct Hlookup_replicas as [replica_host Hlookup_replicas].
+      wp_pures.
+      wp_load.
+      wp_loadField.
+      wp_apply (wp_SliceGet with "[$Hreplicas_sl]").
+      {
+        iPureIntro.
+        replace (int.nat (word.add i 1%Z)) with (int.nat i + 1) by word.
+        done.
+      }
+      iIntros "Hreplicas_sl".
+      wp_apply (wp_MakeClerk with "[]").
+      {
+        instantiate (1:=γsrv').
+        instantiate (1:=γ).
+        admit. (* FIXME: recursive is_pb_host *)
+      }
+      iIntros (ck) "#Hck".
+      wp_load.
+      wp_loadField.
+      wp_apply (wp_SliceSet (V:=loc) with "[$Hclerks_sl]").
+      {
+        iPureIntro.
+        Search "lookup".
+        apply lookup_lt_is_Some_2.
+        word.
+      }
+      iIntros "Hclerks_sl".
+      wp_pures.
+      wp_load.
+      wp_store.
+      iLeft.
+      iModIntro.
+      iSplitR; first done.
+      iFrame "∗".
+
+      destruct clerksLeft.
+      { exfalso. rewrite app_nil_r in Hlen. word. }
+      replace (<[int.nat i:=ck]> (clerksComplete ++ l :: clerksLeft))
+              with
+          (((clerksComplete ++ [ck]) ++ (clerksLeft))); last first.
+      {
+        replace (int.nat i) with (length clerksComplete + 0) by word.
+        rewrite insert_app_r.
+        rewrite -app_assoc.
+        done.
+      }
+
+      iExists _, _, _.
+      iFrame "∗".
+      iSplitL; first iPureIntro.
+      {
+        rewrite app_length /=.
+        word.
+      }
+      iSplitL; first iPureIntro.
+      {
+        rewrite app_length.
+        rewrite app_length.
+        simpl.
+        rewrite app_length in Hlen.
+        rewrite cons_length in Hlen.
+        word.
+      }
+      replace (take (length (clerksComplete ++ [ck])) backupγ)
+              with
+              ((take (length clerksComplete) backupγ) ++ [γsrv']); last first.
+      {
+        rewrite app_length.
+        simpl.
+        rewrite take_more; last first.
+        { word. }
+        f_equal.
+        apply list_eq.
+        intros.
+        destruct i0.
+        {
+          simpl.
+          rewrite lookup_take; last first.
+          { lia. }
+          rewrite lookup_drop.
+          rewrite HcompleteLen.
+          rewrite -H.
+          simpl.
+          rewrite lookup_cons.
+          simpl.
+          destruct (int.nat i + 1).
+          {
+            exfalso.
+            admit.
+          }
+          admit.
+        }
+        admit.
+      }
+      admit.
+    }
+Admitted.
+
+End pb_becomeprimary_proof.
