src/program_proof/simplepb/pb_makeclerk_proof.v
@@ -1,0 +1,31 @@
+From Perennial.program_proof Require Import grove_prelude.
+From Goose.github_com.mit_pdos.gokv.simplepb Require Export pb.
+From Perennial.program_proof.grove_shared Require Import urpc_proof urpc_spec.
+From Perennial.program_proof.simplepb Require Import pb_definitions.
+
+Section pb_makeclerk_proof.
+Context `{!heapGS Σ, !stagedG Σ}.
+Context {pb_record:PBRecord}.
+
+Notation OpType := (pb_OpType pb_record).
+Notation has_op_encoding := (pb_has_op_encoding pb_record).
+Notation has_snap_encoding := (pb_has_snap_encoding pb_record).
+Notation has_op_encoding_injective := (pb_has_op_encoding_injective pb_record).
+Notation compute_reply := (pb_compute_reply pb_record).
+Notation pbG := (pbG (pb_record:=pb_record)).
+
+Context `{!waitgroupG Σ}.
+Context `{!pbG Σ}.
+
+Lemma wp_MakeClerk γ γsrv host :
+{{{
+      is_pb_host γ γsrv host
+}}}
+  MakeClerk #host
+{{{
+      (ck:loc), RET #ck; is_Clerk ck γ γsrv
+}}}.
+Proof.
+Admitted.
+
+End pb_makeclerk_proof.
